@prefix owl: <http://www.w3.org/2002/07/owl#> .
@prefix rdfs: <http://www.w3.org/2000/01/rdf-schema#> .

<http://purl.org/net/vsr/daqar#> a owl:Ontology .
<http://purl.org/net/vsr/daqar#EndValue>
  a owl:ObjectProperty ;
  rdfs:domain <http://purl.org/net/vsr/daqar#FunctionParam> ;
  rdfs:comment "Represents the end value of a function" ;
  rdfs:label "EndValue" .

<http://purl.org/net/vsr/daqar#ReturnType>
  a owl:ObjectProperty, owl:Class ;
  rdfs:domain <http://purl.org/net/vsr/daqar#QualityAssessment>, <http://purl.org/net/vsr/daqar#QualityAssessmentCombination> ;
  rdfs:range <http://purl.org/net/vsr/daqar#ReturnType> ;
  rdfs:label "ReturnType" ;
  rdfs:comment """Indicates the numeric type of the returned assessment result or
Indicates the type of the returned value for the assessment result""" .

<http://purl.org/net/vsr/daqar#ReturnValue>
  a owl:ObjectProperty, owl:Class ;
  rdfs:domain <http://purl.org/net/vsr/daqar#FunctionParam>, <http://purl.org/net/vsr/daqar#QualityAssessment> ;
  rdfs:range <http://purl.org/net/vsr/daqar#ReturnValue> ;
  rdfs:comment """Indicates the computation type of the returned assessment value or
Represents the (constant) return value of a function""" ;
  rdfs:label "ReturnValue" .

<http://purl.org/net/vsr/daqar#StartValue>
  a owl:ObjectProperty ;
  rdfs:domain <http://purl.org/net/vsr/daqar#FunctionParam> ;
  rdfs:comment "Represents the start value of a function" ;
  rdfs:label "StartValue" .

<http://purl.org/net/vsr/daqar#ValueGreaterEqualThan>
  a owl:ObjectProperty ;
  rdfs:domain <http://purl.org/net/vsr/daqar#AssessmentCondition> ;
  rdfs:comment "Indicates what happens if the measured value is greater or euqal than the specified value" ;
  rdfs:label "ValueGreaterEqualThan" .

<http://purl.org/net/vsr/daqar#ValueGreaterThan>
  a owl:ObjectProperty ;
  rdfs:domain <http://purl.org/net/vsr/daqar#AssessmentCondition> ;
  rdfs:comment "Indicates what happens if the measured value is greater than the specified value" ;
  rdfs:label "ValueGreaterThan" .

<http://purl.org/net/vsr/daqar#ValueLowerEqualThan>
  a owl:ObjectProperty ;
  rdfs:domain <http://purl.org/net/vsr/daqar#AssessmentCondition> ;
  rdfs:comment "Indicates what happens if the measured value is lower or euqal than the specified value" ;
  rdfs:label "ValueLowerEqualThan" .

<http://purl.org/net/vsr/daqar#ValueLowerThan>
  a owl:ObjectProperty ;
  rdfs:domain <http://purl.org/net/vsr/daqar#AssessmentCondition> ;
  rdfs:comment "Indicates what happens if the measured value is lower than the specified value" ;
  rdfs:label "ValueLowerThan" .

<http://purl.org/net/vsr/daqar#expectedDataType>
  a owl:ObjectProperty ;
  rdfs:domain <http://purl.org/net/vsr/daqar#QualityRequirement> ;
  rdfs:comment "Indicates the expected return type of the measurement result" ;
  rdfs:label "expectedDataType" .

<http://purl.org/net/vsr/daqar#hasAssessment>
  a owl:ObjectProperty ;
  rdfs:domain <http://purl.org/net/vsr/daqar#QualityAssessmentTerm>, <http://purl.org/net/vsr/daqar#QualityRequirement>, <http://purl.org/net/vsr/daqar#QualityRequirementSpec> ;
  rdfs:range <http://purl.org/net/vsr/daqar#QualityAssessment>, <http://purl.org/net/vsr/daqar#QualityAssessmentCombination> ;
  rdfs:comment """Indicates the definition of an overall assessment relation how the quality of a data source has to be calculated or
Indicates a quality assessment that shall be calculated or
Indicates a calculation function for assessing the measurement result""" ;
  rdfs:label "hasAssessment" .

<http://purl.org/net/vsr/daqar#hasAssessmentFunction>
  a owl:ObjectProperty ;
  rdfs:domain <http://purl.org/net/vsr/daqar#AssessmentCondition> ;
  rdfs:range <http://purl.org/net/vsr/daqar#AssessmentFunction> ;
  rdfs:comment "Defines a mapping function how to represent the measured value as an assessment value" ;
  rdfs:label "hasAssessmentFunction" .

<http://purl.org/net/vsr/daqar#hasAssessmentParam>
  a owl:ObjectProperty ;
  rdfs:domain <http://purl.org/net/vsr/daqar#QualityRequirement> ;
  rdfs:range <http://purl.org/net/vsr/daqar#AssessmentParam> ;
  rdfs:comment "Specifies parameter values that can be used in combination with well-known assessment function definitions." ;
  rdfs:label "hasAssessmentParam" .

<http://purl.org/net/vsr/daqar#hasAssessmentTerms>
  a owl:ObjectProperty ;
  rdfs:domain <http://purl.org/net/vsr/daqar#QualityAssessmentCombination> ;
  rdfs:range <http://purl.org/net/vsr/daqar#QualityAssessmentTerm> ;
  rdfs:comment "Represents a list of independent QualityAssessment subcalculations that should be combined to an overall assessment result" ;
  rdfs:label "hasAssessmentTerms" .

<http://purl.org/net/vsr/daqar#hasCondition>
  a owl:ObjectProperty ;
  rdfs:domain <http://purl.org/net/vsr/daqar#QualityAssessment> ;
  rdfs:range <http://purl.org/net/vsr/daqar#AssessmentCondition> ;
  rdfs:comment "Specifies an operation or a condition that has to be met by the measured value in order to calculate an assessment result" ;
  rdfs:label "hasCondition" .

<http://purl.org/net/vsr/daqar#hasFunctionParam>
  a owl:ObjectProperty ;
  rdfs:domain <http://purl.org/net/vsr/daqar#AssessmentFunction> ;
  rdfs:comment "Defines values for the functional parameters required by dqr:FunctionType" ;
  rdfs:label "hasFunctionParam" .

<http://purl.org/net/vsr/daqar#hasFunctionType>
  a owl:ObjectProperty ;
  rdfs:domain <http://purl.org/net/vsr/daqar#AssessmentFunction> ;
  rdfs:range <http://purl.org/net/vsr/daqar#FunctionType> ;
  rdfs:comment "Indicates the functional type of the calculation" ;
  rdfs:label "hasFunctionType" .

<http://purl.org/net/vsr/daqar#hasImplementation>
  a owl:ObjectProperty ;
  rdfs:domain <http://purl.org/net/vsr/daqar#QualityRequirement> ;
  rdfs:comment "Indicates if the calculation relies on a concrete, mandatory implementation of a quality requirement concept" ;
  rdfs:label "hasImplementation" .

<http://purl.org/net/vsr/daqar#hasParamType>
  a owl:ObjectProperty ;
  rdfs:domain <http://purl.org/net/vsr/daqar#AssessmentParam> ;
  rdfs:comment "Indicates the type of the assessment param" ;
  rdfs:label "hasParamType" .

<http://purl.org/net/vsr/daqar#hasRequirementConcept>
  a owl:ObjectProperty ;
  rdfs:domain <http://purl.org/net/vsr/daqar#QualityRequirement> ;
  rdfs:comment """Represents the particular quality concepts in form of a URI
This can be a daq:Metric, a dqv:Metric, a SHACL URL or any other URI representing a quality requirement""" ;
  rdfs:label "hasRequirementConcept" .

<http://purl.org/net/vsr/daqar#hasRequirementType>
  a owl:ObjectProperty ;
  rdfs:domain <http://purl.org/net/vsr/daqar#QualityRequirement> ;
  rdfs:range <http://purl.org/net/vsr/daqar#RequirementType> ;
  rdfs:comment "Indicates the type of examined quality aspect" ;
  rdfs:label "hasRequirementType" .

<http://purl.org/net/vsr/daqar#hasRequirements>
  a owl:ObjectProperty ;
  rdfs:domain <http://purl.org/net/vsr/daqar#QualityRequirementSpec> ;
  rdfs:range <http://purl.org/net/vsr/daqar#QualityRequirement> ;
  rdfs:comment "Indicates the QualityRequirements that have to be checked" ;
  rdfs:label "hasRequirements" .

<http://purl.org/net/vsr/daqar#hasUnit>
  a owl:ObjectProperty ;
  rdfs:domain <http://purl.org/net/vsr/daqar#QualityRequirement> ;
  rdfs:comment "Indicates the unit of the measurement result" ;
  rdfs:label "hasUnit" .

<http://purl.org/net/vsr/daqar#hasValue>
  a owl:ObjectProperty ;
  rdfs:domain <http://purl.org/net/vsr/daqar#AssessmentParam> ;
  rdfs:comment "Specified the value of the assessment parameter" ;
  rdfs:label "hasValue" .

<http://purl.org/net/vsr/daqar#hasWeight>
  a owl:ObjectProperty ;
  rdfs:domain <http://purl.org/net/vsr/daqar#QualityAssessmentTerm> ;
  rdfs:comment "Indicates the influence of the current assessment to the overall assessment score" ;
  rdfs:label "hasWeight" .

<http://purl.org/net/vsr/daqar#AssessmentCondition>
  a owl:Class ;
  rdfs:comment "Represents a measurement value range and a mapping function to an assessment value" ;
  rdfs:label "AssessmentCondition" .

<http://purl.org/net/vsr/daqar#AssessmentFunction>
  a owl:Class ;
  rdfs:comment "Represents a mapping function to map an actual measurement value to a corrresponding assessment value" ;
  rdfs:label "AssessmentFunction" .

<http://purl.org/net/vsr/daqar#AssessmentParam>
  a owl:Class ;
  rdfs:comment "Represents a parameter with a defined value that can be reused by an assessment tool in combination with a well-known dqr:Assessment function" ;
  rdfs:label "AsssessmentParam" .

<http://purl.org/net/vsr/daqar#AverageParam>
  a owl:Class ;
  rdfs:subClassOf <http://purl.org/net/vsr/daqar#ParamType> .

<http://purl.org/net/vsr/daqar#ConstantFunction>
  a owl:Class ;
  rdfs:subClassOf <http://purl.org/net/vsr/daqar#FunctionType> ;
  rdfs:comment "A mapping function defined through a constant dqr:ReturnValue" ;
  rdfs:label "ConstantFunction" .

<http://purl.org/net/vsr/daqar#ConstantValue>
  a owl:Class ;
  rdfs:subClassOf <http://purl.org/net/vsr/daqar#ReturnValue> ;
  rdfs:comment "A constant ReturnValue" ;
  rdfs:label "ConstantValue" .

<http://purl.org/net/vsr/daqar#CustomFunction>
  a owl:Class ;
  rdfs:subClassOf <http://purl.org/net/vsr/daqar#FunctionType> ;
  rdfs:comment "A custom defined mapping function defined through a dqr:CustomFunctionTerm" ;
  rdfs:label "CustomFunction" .

<http://purl.org/net/vsr/daqar#FunctionParam>
  a owl:Class ;
  rdfs:comment "Represents a bound value used by a dqr:FunctionType function for calculation purposes" ;
  rdfs:label "FunctionParam" .

<http://purl.org/net/vsr/daqar#FunctionType>
  a owl:Class ;
  rdfs:comment "The mathematical function how to map a measured value to an assessment value" ;
  rdfs:label "FunctionType" .

<http://purl.org/net/vsr/daqar#FunctionalValue>
  a owl:Class ;
  rdfs:subClassOf <http://purl.org/net/vsr/daqar#ReturnValue> ;
  rdfs:comment "A ReturnValue described through a Function" ;
  rdfs:label "FunctionalValue" .

<http://purl.org/net/vsr/daqar#GreaterEqualThanParam>
  a owl:Class ;
  rdfs:subClassOf <http://purl.org/net/vsr/daqar#ParamType> .

<http://purl.org/net/vsr/daqar#GreaterThanParam>
  a owl:Class ;
  rdfs:subClassOf <http://purl.org/net/vsr/daqar#ParamType> .

<http://purl.org/net/vsr/daqar#LinearFunction>
  a owl:Class ;
  rdfs:subClassOf <http://purl.org/net/vsr/daqar#FunctionType> ;
  rdfs:comment "A mapping function defined through a dqr:StartValue and dqr:EndValue" ;
  rdfs:label "LinearFunction" .

<http://purl.org/net/vsr/daqar#LowerEqualThanParam>
  a owl:Class ;
  rdfs:subClassOf <http://purl.org/net/vsr/daqar#ParamType> .

<http://purl.org/net/vsr/daqar#LowerThanParam>
  a owl:Class ;
  rdfs:subClassOf <http://purl.org/net/vsr/daqar#ParamType> .

<http://purl.org/net/vsr/daqar#ParamType> a owl:Class .
<http://purl.org/net/vsr/daqar#QualityAssessment>
  a owl:Class ;
  rdfs:comment "Represents the defintion of a function of measurement boundaries on how to assess the measured value of a related quality concept of interest" ;
  rdfs:label "QualityAssessment" .

<http://purl.org/net/vsr/daqar#QualityAssessmentCombination>
  a owl:Class ;
  rdfs:comment "Represents an instruction on how to combine the results from multiple dqr:QualityAssessments to an overall assessment score" ;
  rdfs:label "QualityAssessmentCombination" .

<http://purl.org/net/vsr/daqar#QualityAssessmentTerm>
  a owl:Class ;
  rdfs:comment "Represents a weighted assessment sub-calculation for a particular requirement" ;
  rdfs:label "QualityAssessmentTerm" .

<http://purl.org/net/vsr/daqar#QualityGrade>
  a owl:Class ;
  rdfs:subClassOf <http://purl.org/net/vsr/daqar#ReturnType> ;
  rdfs:label "QualityGrade", "ReturnType for an integer representation 1 (best) <= DQ <= 6 (worst)" .

<http://purl.org/net/vsr/daqar#QualityRatio>
  a owl:Class ;
  rdfs:subClassOf <http://purl.org/net/vsr/daqar#ReturnType> ;
  rdfs:comment "ReturnType for a decimal representation 0.0 (worst) <= DQ <= 1.0 (best)" ;
  rdfs:label "QualityRatio" .

<http://purl.org/net/vsr/daqar#QualityRequirement>
  a owl:Class ;
  rdfs:comment "Represents a particular measurable quality aspect of interest whose result is assesseable" ;
  rdfs:label "QualityRequirement" .

<http://purl.org/net/vsr/daqar#QualityRequirementSpec>
  a owl:Class ;
  rdfs:comment "Represents a specification of requirements on a data set or data service from consumer side for quality assessment purposes" ;
  rdfs:label "QualityRequirementSpec" .

<http://purl.org/net/vsr/daqar#QualityStar>
  a owl:Class ;
  rdfs:subClassOf <http://purl.org/net/vsr/daqar#ReturnType> ;
  rdfs:comment "ReturnType for an integer representation 0 (worst) <= DQ <= 5 (best)" ;
  rdfs:label "QualityStar" .

<http://purl.org/net/vsr/daqar#RequirementType>
  a owl:Class ;
  rdfs:comment "Indicates the type of examined quality aspect" ;
  rdfs:label "RequirementType" .

<http://purl.org/net/vsr/daqar#ShapeConstraint>
  a owl:Class ;
  rdfs:subClassOf <http://purl.org/net/vsr/daqar#RequirementType> ;
  rdfs:comment "a RequirementType for SHACL-like template graph descriptors that are run by a separate processor" ;
  rdfs:label "ShapeConstraint" .

<http://purl.org/net/vsr/daqar#SimpleMetric>
  a owl:Class ;
  rdfs:subClassOf <http://purl.org/net/vsr/daqar#RequirementType> ;
  rdfs:comment "a RequirementType for directly calculable metrics such as DQV, daq or ISO metrics" ;
  rdfs:label "SimpleMetric" .

